theories/DSub/syn/ds_rules.v
@@ -30,15 +30,15 @@ Section lang_rules.
     intros ?; apply nsteps_once, pure_head_step_pure_step;
       constructor; [solve_exec_safe | solve_exec_puredet].
 
-  Global Instance pure_lam e1 v2 :
+  #[global] Instance pure_lam e1 v2 :
     PureExec True 1 (tapp (tv (vabs e1)) (tv v2)) e1.|[v2 /].
   Proof. solve_pure_exec. Qed.
 
-  Global Instance pure_tskip v:
+  #[global] Instance pure_tskip v:
     PureExec True 1 (tskip (tv v)) (tv v).
   Proof. solve_pure_exec. Qed.
 
-  Global Instance pure_tskip_iter v i:
+  #[global] Instance pure_tskip_iter v i:
     PureExec True i (iterate tskip i (tv v)) (tv v).
   Proof.
     move => _. elim: i => [|i IHi]; rewrite ?iterate_0 ?iterate_S //. by repeat constructor.
