theories/Dot/examples/ex_utils.v
@@ -58,8 +58,8 @@ Notation "'val' l = v" := (l, dpt v) (at level 60, l at level 50).
 Notation "'type' l = T" := (l, dtysyn T) (at level 60, l at level 50).
 
 (** Notation for object types. *)
-Global Instance: Top ty := TTop.
-Global Instance: Bottom ty := TBot.
+#[global] Instance: Top ty := TTop.
+#[global] Instance: Bottom ty := TBot.
 
 Open Scope ty_scope.
 Notation "{@ T1 }" := ( TAnd T1 ⊤ ) (format "{@  T1  }"): ty_scope.
