theories/Dot/syn/rules.v
@@ -40,35 +40,35 @@ Section lang_rules.
     intros ?; apply nsteps_once, pure_head_step_pure_step;
       constructor; [solve_exec_safe | solve_exec_puredet].
 
-  Global Instance pure_lam e1 v2 :
+  #[global] Instance pure_lam e1 v2 :
     PureExec True 1 (tapp (tv (vabs e1)) (tv v2)) e1.|[v2 /].
   Proof. solve_pure_exec. Qed.
 
-  Global Instance pure_tproj l v p :
+  #[global] Instance pure_tproj l v p :
     PureExec (v @ l ↘ dpt p) 1 (tproj (tv v) l) (path2tm p).
   Proof. solve_pure_exec. Qed.
 
-  Global Instance pure_tskip v:
+  #[global] Instance pure_tskip v:
     PureExec True 1 (tskip (tv v)) (tv v).
   Proof. solve_pure_exec. Qed.
 
-  Global Instance pure_tif_true t1 t2:
+  #[global] Instance pure_tif_true t1 t2:
     PureExec True 1 (tif (tv $ vbool true) t1 t2) t1.
   Proof. solve_pure_exec. Qed.
 
-  Global Instance pure_tif_false t1 t2:
+  #[global] Instance pure_tif_false t1 t2:
     PureExec True 1 (tif (tv $ vbool false) t1 t2) t2.
   Proof. solve_pure_exec. Qed.
 
-  Global Instance pure_unop u v v' :
+  #[global] Instance pure_unop u v v' :
     PureExec (un_op_eval u v = Some v') 1 (tun u (tv v)) (tv v').
   Proof. solve_pure_exec. Qed.
 
-  Global Instance pure_binop b v1 v2 v' :
+  #[global] Instance pure_binop b v1 v2 v' :
     PureExec (bin_op_eval b v1 v2 = Some v') 1 (tbin b (tv v1) (tv v2)) (tv v').
   Proof. solve_pure_exec. Qed.
 
-  Global Instance pure_tskip_iter v i:
+  #[global] Instance pure_tskip_iter v i:
     PureExec True i (iterate tskip i (tv v)) (tv v).
   Proof.
     move => _. elim: i => [|i IHi]; rewrite ?iterate_0 ?iterate_S //. by repeat constructor.
